Lax version of well-formedness for readers and resources.
Most code deals with unknown keys. The specification for these functions must
cover the case where the keys are owned by the attacker. To allow this, we
generalize the well-formedness condition on resources so that it allows the
attacker to be a private reader.

crypto1.v
@@ -179,6 +179,12 @@ Proof.
 case: r=> [?|?[|?]?|[|?]?] //=; set_solver.
 Qed.
 
+Definition pub_dec_key r : Prop :=
+  match r with
+  | RAKey _ RPub _ | RSKey RPub _ => True
+  | _ => False
+  end.
+
 Class resG := {
   res_inG :> inG Σ (agreeR resO);
 }.
@@ -272,30 +278,70 @@ Qed.
 Definition priv_keysT rs_priv : iProp Σ :=
   ∀ l, ⌜l ∈ rs_priv⌝ -∗ priv_keyT rs_priv l.
 
-Definition wf_readers rs : iProp Σ :=
+Definition pub_keyT l : iProp Σ :=
+  ∃ r, pre_resT r l ∗ ⌜pub_dec_key r⌝.
+
+Global Instance pub_keyT_persistent l : Persistent (pub_keyT l).
+Proof. apply _. Qed.
+
+Global Instance pub_keyT_timeless l : Timeless (pub_keyT l).
+Proof.
+rewrite /Timeless /pub_keyT bi.later_exist_except_0.
+iMod 1 as (r) "[#Hown >%Hpriv]".
+iMod (later_pre_resT with "Hown") as (r') "[Hown' He]".
+iExists r'; iSplit; eauto; rewrite res_equivI.
+case: r Hpriv => [rs|rs_enc [|rs_dec] Φ|[|rs_dec] Φ] //= Hpriv;
+case: r'=> [?|???|??]; try by iDestruct "He" as "> []".
+- by iDestruct "He" as "(><-&><-&?)".
+- by iDestruct "He" as "(><-&?)".
+Qed.
+
+Definition pub_keysT (rs_pub : gset loc) : iProp Σ :=
+  ∀ l, ⌜l ∈ rs_pub⌝ -∗ pub_keyT l.
+
+Global Instance pub_keysT_persistent rs_pub : Persistent (pub_keysT rs_pub).
+Proof. apply _. Qed.
+
+Global Instance pub_keysT_timeless rs_pub : Timeless (pub_keysT rs_pub).
+Proof. apply _. Qed.
+
+Definition wf_readers_priv rs : iProp Σ :=
   ∃ rs_priv, priv_keysT rs_priv ∗ ⌜pre_wf_readers rs_priv rs⌝.
 
-Global Instance wf_readers_persistent rs : Persistent (wf_readers rs).
+Global Instance wf_readers_priv_persistent rs : Persistent (wf_readers_priv rs).
 Proof. apply _. Qed.
+
+Global Instance wf_readers_priv_timeless rs : Timeless (wf_readers_priv rs).
+Proof. apply _. Qed.
+
+Definition wf_readers rs : iProp Σ :=
+  match rs with
+  | RPub => True
+  | RPriv rs =>
+    ∃ rs1 rs2, ⌜rs = rs1 ∪ rs2⌝ ∗ wf_readers_priv (RPriv rs1) ∗ pub_keysT rs2
+  end.
+
+Global Instance wf_readers_persistent rs : Persistent (wf_readers rs).
+Proof. case: rs=> *; apply _. Qed.
 
 Global Instance wf_readers_timeless rs : Timeless (wf_readers rs).
-Proof. apply _. Qed.
+Proof. case: rs=> *; apply _. Qed.
 
-Definition wf_res r : iProp Σ :=
+Definition wf_res_priv r : iProp Σ :=
   ∃ rs_priv, priv_keysT rs_priv ∗ ⌜pre_wf_res rs_priv r⌝.
 
-Global Instance wf_res_persistent r : Persistent (wf_res r).
+Global Instance wf_res_priv_persistent r : Persistent (wf_res_priv r).
 Proof. apply _. Qed.
 
-Global Instance wf_res_timeless r : Timeless (wf_res r).
+Global Instance wf_res_priv_timeless r : Timeless (wf_res_priv r).
 Proof. apply _. Qed.
 
-Lemma wf_resE r :
-  wf_res r ⊣⊢@{iPropI Σ}
+Lemma wf_res_privE r :
+  wf_res_priv r ⊣⊢@{iPropI Σ}
   match r with
-  | RNonce rs => wf_readers rs
-  | RAKey rs_enc rs_dec _ => wf_readers rs_enc ∧ wf_readers rs_dec
-  | RSKey rs _ => wf_readers rs
+  | RNonce rs => wf_readers_priv rs
+  | RAKey rs_enc rs_dec _ => wf_readers_priv rs_enc ∧ wf_readers_priv rs_dec
+  | RSKey rs _ => wf_readers_priv rs
   end.
 Proof.
 case: r; try by move=> *; iSplit; eauto.
@@ -315,6 +361,30 @@ move=> rs_enc rs_dec Φ /=; iSplit.
     iApply (priv_keyT_sub with "Hpriv_dec"); set_solver.
 Qed.
 
+Definition res_privT r l : iProp Σ :=
+  pre_resT r l ∗ wf_res_priv r.
+
+Lemma res_privT_agree r1 r2 l : res_privT r1 l -∗ res_privT r2 l -∗ r1 ≡ r2.
+Proof.
+iIntros "[Hr1 _] [Hr2 _]". iApply (pre_resT_agree with "Hr1 Hr2").
+Qed.
+
+Global Instance res_privT_persistent r l : Persistent (res_privT r l).
+Proof. apply _. Qed.
+
+Definition wf_res r : iProp Σ :=
+  match r with
+  | RNonce rs => wf_readers rs
+  | RAKey rs_enc rs_dec _ => wf_readers rs_enc ∧ wf_readers rs_dec
+  | RSKey rs _ => wf_readers rs
+  end.
+
+Global Instance wf_resT_persistent r : Persistent (wf_res r).
+Proof. case: r=> *; apply _. Qed.
+
+Global Instance wf_resT_timeless r : Timeless (wf_res r).
+Proof. case: r=> *; apply _. Qed.
+
 Definition resT r l : iProp Σ :=
   pre_resT r l ∗ wf_res r.
 
@@ -324,7 +394,7 @@ iIntros "[Hr1 _] [Hr2 _]". iApply (pre_resT_agree with "Hr1 Hr2").
 Qed.
 
 Global Instance resT_persistent r l : Persistent (resT r l).
-Proof. apply _. Qed.
+Proof. case: r=> *; apply _. Qed.
 
 Definition nonceT rs l : iProp Σ := resT (RNonce rs) l.
 
@@ -436,6 +506,12 @@ Definition stermT rs t : iProp Σ :=
 Global Instance stermT_persistent rs t : Persistent (stermT rs t).
 Proof. apply _. Qed.
 
+Definition termT' rs t : iProp Σ :=
+  termT rs t ∨ ∃ l, ⌜l ∈ rs⌝ ∗ pub_keyT l ∗ termT RPub t.
+
+Definition stermT' rs t : iProp Σ :=
+  stermT rs t ∨ ∃ l, ⌜l ∈ rs⌝ ∗ pub_keyT l ∗ termT RPub t.
+
 (** Because of [sub_termT], the definition of [termT] does not allow us to track
 the owners of a term exactly.  To remedy that, we introduce the [secretT rs t]
 predicate below, which says that [t] is private exactly to the readers in
@@ -479,5 +555,7 @@ Arguments RNonce {_} _.
 Arguments nonceT {_ _ _} _ _.
 Arguments skeyT {_ _ _} _ _ _.
 Arguments akeyT {_ _ _} _ _ _ _.
+Arguments wf_readers_priv {_ _ _} _.
 Arguments wf_readers {_ _ _} _.
+Arguments wf_res_priv {_ _ _} _.
 Arguments wf_res {_ _ _} _.
